Logic/FirstOrder/Computability/Calculus.lean
@@ -176,13 +176,13 @@ lemma isProper_append {l₁ l₂ : ProofList L} (h₁ : isProper l₁) (h₂ : i
   · simpa
   · simp
     rcases c with ⟨⟨⟩, Γ⟩ <;> simp[isProper] at h₁ ⊢
-    case axL k r v => { exact ⟨⟨ih h₁.1.1, h₁.1.2⟩, h₁.2⟩ }
-    case verum => { exact ⟨ih h₁.1, h₁.2⟩ }
-    case and p q => { exact ⟨⟨⟨ih h₁.1.1.1, h₁.1.1.2⟩, Or.inl h₁.1.2⟩, Or.inl h₁.2⟩ }
-    case or p q => { exact ⟨⟨ih h₁.1.1, h₁.1.2⟩, Or.inl h₁.2⟩ }
-    case all => { exact ⟨⟨ih h₁.1.1, h₁.1.2⟩, Or.inl h₁.2⟩ }
-    case ex => { exact ⟨⟨ih h₁.1.1, h₁.1.2⟩, Or.inl h₁.2⟩ }
-    case wk => { exact ⟨⟨ih h₁.1.1, h₁.1.2⟩, Or.inl h₁.2⟩ }
+    case axL k r v => exact ⟨⟨ih h₁.1.1, h₁.1.2⟩, h₁.2⟩
+    case verum => exact ⟨ih h₁.1, h₁.2⟩
+    case and p q => exact ⟨⟨⟨ih h₁.1.1.1, h₁.1.1.2⟩, Or.inl h₁.1.2⟩, Or.inl h₁.2⟩
+    case or p q => exact ⟨⟨ih h₁.1.1, h₁.1.2⟩, Or.inl h₁.2⟩
+    case all => exact ⟨⟨ih h₁.1.1, h₁.1.2⟩, Or.inl h₁.2⟩
+    case ex => exact ⟨⟨ih h₁.1.1, h₁.1.2⟩, Or.inl h₁.2⟩
+    case wk => exact ⟨⟨ih h₁.1.1, h₁.1.2⟩, Or.inl h₁.2⟩
 
 open Derivation
 
@@ -351,7 +351,6 @@ lemma provable_iff_isProofFn {T : Theory L} [DecidablePred T] {σ : Sentence L} 
   · simp; intro e
     rcases decode e.unpair.1 with (_ | ⟨l⟩) <;> simp
     rcases decode e.unpair.2 with (_ | ⟨U⟩) <;> simp
-    simp only [Bool.cond_eq_ite, Bool.and_eq_true, ite_eq_iff]; simp
     intro h₁ h₂ h₃
     exact ⟨l, U, h₁, h₂, h₃⟩
 
